\section{Mathe Grundlagen}	

	\subsection{Partialbruchzerlegung}
		\input{Content/Rechenregeln/PBZ}
			
	\subsection{Trigonometrie}
		\input{Content/Rechenregeln/Trigo}	

	\subsection{Differentialrechnung}
		$f'(x_0)=\lim\limits_{\Delta x\rightarrow 0} \frac{f(x_0+\Delta) x-f(x_0)}{\Delta x}$	
		
		Kettenregel: $\frac{d f(g(x))}{dx} = f'(g(x)) \cdot g'(x)$
			
	\subsection{Taylor Polynom}
		$f(x_0+h)=f(x_0) + f'(x_0)h + \frac{f''(x_0)}{2}h^2 + \frac{f'''(x_0)}{3!}h^3 + \ldots + \frac{f^{(n)}(x_0)}{n!}h^n + R_n(x_0, h)$

	\subsection{Integralrechnung}	
	\begin{tabbing}
	     xxxxxxxxxxxxxxxxxxxxxxxxxxxxxxx \= xxx \= xxxxxxxxxxxxxxxxxxxxxxxxxxxxxxxxxxxxxxxxxxxxxxxxxxxxxxx\kill  
	     Integration\>\>$A=\int\limits_{a}^{b}{f(t)dt}=\left[F(t)\right]_a^b=F(b)-F(a)$\\[0.2cm]
	     Linearität\>		  
	   $\qquad\int{f(\alpha x+\beta )dx=\frac{1}{\alpha}\cdot F(\alpha x+
				\beta)+C}$\\[0.2cm]
		   Partielle Integration\>
	   $\qquad\int\limits_a^b{\underset{\Uparrow}{u}'(x)\cdot \underset{\Downarrow}{v}(x)dx}=\biggl[ u(x)\cdot v(x) \biggr]_a^b
	   -\int\limits_a^b{u(x)\cdot v'(x)dx}$\\[0.2cm]
	   Substitution (Rationalisierung)\>
	   $\qquad t=\tan\frac{x}{2}, \qquad dx=\frac{2dt}{1+t^2} \qquad 
	   \sin  x=\frac{2t}{1+t^2} \qquad \cos x=\frac{1-t^2}{1+t^2}
				\quad\int{R(\sin(x)\cos(x))dx}$\\ 
	   Allgemeine Substitution \> \>
				$\int\limits_{a}^{b}{f(x)dx}=\int\limits_{g^{-1}(a)}^{g^{-1}(b)}{f(g(t))\cdot
				g'(t)dt}\qquad t=g^{-1}(x)\qquad  \fbox{x=g(t)}\qquad dx=g'(t)\cdot dt$\\
	   Logarithmische Integration \>\>
	    $ \int{\frac{f'(x)}{f(x)}dx}=\ln|f(x)|+C	\qquad{(f(x)\neq 1)}$\\[0.2cm]
	  Spezielle Form des Integranden \>\>
		 		$\int{f'(x)\cdot (f(x))^{\alpha} dx}= f(x)^{\alpha +1}\cdot
		 		\frac{1}{\alpha+1}+C \qquad{(\alpha \neq -1)}$\\ 
	   Differentiation\>\>
		 		$\int \limits ^{b} _{a} {f'(t)dt}=f(b)-f(a)$\qquad
				$\frac{d}{dx} \int \limits ^{x} _{1} {f(t)dt}=f(x)$
	\end{tabbing}
	%\subsubsection{Einige unbestimmte Integrale}
	\includegraphics[width=19cm]{Content/Rechenregeln/integrale.png} 
	
	
			
	\subsection{Differentialgleichungen}
		\input{Content/Rechenregeln/DGL}
	\subsection{DifferentialRechnung}
		\begin{tabular}{llll}
			Kettenregel:	& $f\big(g(x)\big)$ &$=$ & $g'(x)\cdot f'\big(g(x)\big)$\\[0.1cm]
			Produktregel:	& $f(x)\cdot g(x)$ &$=$ & $f'(x)\cdot g(x) + f(x)\cdot g'(x)$\\[0.1cm]
			Quotientenregel:& $\frac{f(x)}{g(x)}$ &$=$ & $\frac{f'(x)g(x)-f(x)g'(x)}{g^2(x)}$\\
		\end{tabular}
	\subsection{Divers}	
	\begin{minipage}[t]{9.5cm}
		\subsubsection{Quadratische Lösungsformel}
			$ax^2+bx+c=0\quad\Rightarrow\quad x_{1,2}=\frac{-b\pm\sqrt{b^2-4ac}}{2a}$
	\end{minipage}
	\hfill
	\begin{minipage}[t]{9.5cm}
		\subsubsection{Determinanten}
			$\det\left(
			\begin{bmatrix}
				a_{11}&a_{12}\\
				a_{21}&a_{22}\\
			\end{bmatrix}\right)=
			\begin{vmatrix}
				a_{11}&a_{12}\\
				a_{21}&a_{22}\\
			\end{vmatrix}=a_{11}a_{22}-a_{12}a_{21}$
	\end{minipage}\\
	
	
	\begin{minipage}[t]{9.5cm}
		\subsubsection{Matrizeninversion}
			$A=\begin{bmatrix}
						a_{11}&a_{12}\\
						a_{21}&a_{22}\\
				\end{bmatrix}\quad\Rightarrow\quad
			A^{-1}=\frac{1}{det(A)}
			\begin{bmatrix}
				a_{22}&-a_{12}\\
				-a_{21}&a_{11}\\
			\end{bmatrix}$
	\end{minipage}
	\hfill
	\begin{minipage}[t]{9.5cm}
		\subsubsection{Eigenwerte/ Eigenvektoren}
			Eigenwert: $\det(A-\lambda I)\quad\Rightarrow\quad \lambda i$\\
			Eigenvektor: $(A-\lambda_i I)v=0\quad\Rightarrow\quad v_i\qquad(\text{Für jedes }\lambda_i)$\\
			Definition: $ A\cdot \underline{v} = \lambda \cdot \underline{v} $
	\end{minipage}
	
	
	\begin{minipage}[t]{9.5cm}
		\subsubsection{TI-89}
			Gleichung für mehrere Werte:\\
			$(3x+y^2) \mid x=1 \text{ and } y=2 \to Resultat$ 
	\end{minipage}
	
